\date{}
\documentclass[fleqn, a4paper]{article}
\usepackage[top=1in, left=1in, right=1in, bottom=1in]{geometry}
\usepackage{amsmath, amssymb, commath}
\usepackage{gensymb}
\usepackage{tikz, pgfplots}
\usepackage{datetime}
\usepackage{ulem}
\usepackage{xfrac}
\usepackage{enumerate}
%\usepackage{background}
\setcounter{secnumdepth}{4}
\newcommand\numberthis{\addtocounter{equation}{1}\tag{\theequation}}
\renewcommand{\thesubsection}{(\alph{subsection})}
\renewcommand{\thesection}{(\arabic{section})}


%opening
\title{Differential and Integral Methods - Exercise 8}
\author{Aakash Jog\\
	ID: 989323563}
%\date{\formatdate{24}{12}{2014}}

\begin{document}
	
\maketitle
\setlength{\mathindent}{0pt}

%\tableofcontents

\section{Solve the following integrals}

\subsection{\[\int \dfrac{e^x}{1 + e^x} \dif x\]}

Let
\begin{align*}
	t &= 1 + e^x\\
	\therefore \dif t &= e^t	
\end{align*}

\begin{align*}
	\therefore \int \dfrac{e^x}{1 + e^x} \dif x &= \int \dfrac{\dif t}{t}\\
	&= \ln t + c\\
	&= \ln (1 + e^x) + c
\end{align*}

\subsection{\[\int \dfrac{1}{1 + e^x} \dif x\]}

\begin{align*}
	\int \dfrac{1}{1 + e^x} \dif x &= \int \dfrac{1 + e^x}{1 + e^x} \dif x - \int \dfrac{e^x}{1 + e^x} \dif x\\
	&= \int \dif x - \int \dfrac{e^x}{1 + e^x} \dif x
\end{align*}

Let
\begin{align*}
	t &= 1 + e^x\\
	\therefore \dif t &= e^x
\end{align*}

\begin{align*}
	\therefore \int \dfrac{1}{1 + e^x} \dif x &= x - \int \dfrac{\dif t}{t} + c\\
	\therefore \int \dfrac{1}{1 + e^x} \dif x &= x - \ln t + c\\
		\therefore \int \dfrac{1}{1 + e^x} \dif x &= x - \ln (1 + e^x) + c
\end{align*}

\subsection{\[\int \dfrac{5x + 4}{(x-1)(x-2)}\dif x\]}

\begin{align*}
	\int \dfrac{5x + 4}{(x-1)(x-2)}\dif x &= \int \dfrac{5x -5 + 9}{(x-1)(x-2)}\dif x\\
	&= \int \dfrac{5(x - 1) + 9}{(x-1)(x-2)}\dif x\\
	&= \int \left( \dfrac{3}{x - 1} + \dfrac{2}{x + 2} \right) \dif x\\
	&= 3 \ln |x - 1| + 2 \ln |x + 2| + c
\end{align*}

\subsection{\[\int \dfrac{5x^2 - 7x + 3}{x(x - 1)^2} \dif x\]}

\begin{align*}
	\int \dfrac{5x^2 - 7x + 3}{x(x - 1)^2} \dif x &= \int \left( \dfrac{3}{x} + \dfrac{2}{x - 1} + \dfrac{1}{(x - 1)^2} \right)\dif x\\
	&= 3 \ln |x| + 2 \ln |x - 1| - \dfrac{1}{x - 1} + c 
\end{align*}

\subsection{\[\int \dfrac{2x^2 - 2x - 2}{x^3 - x} \dif x\]}

\begin{align*}
	\int \dfrac{2x^2 - 2x - 2}{x^3 - x} \dif x &= \int \dfrac{2x^2 - 2x - 2}{x (x + 1)(x - 1)} \dif x\\
	&= \int \left( \dfrac{2}{x} - \dfrac{1}{x - 1} + \dfrac{1}{x + 1} \right) \dif x\\
	&= 2 \ln |x| - \ln |x - 1| + \ln |x + 1| + c\\
	&= \ln \left\lvert \dfrac{x^2(x+1)}{x - 1} \right\rvert + c
\end{align*}

\section{Write as a sum of simple rational functions \[f(x) = \dfrac{x - 1}{(x^2 + 1)(x + 1)}\]}

Let
\begin{align*}
	f(x) &= \dfrac{Ax + B}{x^2 + 1} + \dfrac{C}{x + 1}\\
	\therefore f(x) &= \dfrac{(Ax + B)(x + 1) + C(x^2 + 1)}{(x^2 + 1)(x + 1)}\\
	&= \dfrac{Ax^2 + (A + B)x + B + Cx^2 + C}{(x^2 + 1)(x + 1)}\\
	&= \dfrac{x^2 (A + C) + x(A + B) + C}{(x^2 + 1)(x + 1)}
\end{align*}
Therefore,
\begin{align*}
	A + B &= 1\\
	A + C &= 0\\
	C &= -1
\end{align*}
\begin{align*}
	\therefore A &= 1 &;& & B &= 0 &;& & C &= -1
\end{align*}
Therefore,
\begin{align*}
	f(x) &= \dfrac{x}{x^2 + 1} - \dfrac{1}{x + 1}
\end{align*}

\section{Solve the following integrals}

\subsection{\[\int (1 + \sqrt[3]{x^2})^2 \dif x\]}

Let
\begin{align*}
	x &= t^3\\
	\therefore \dif x &= 3t^2 \dif t
\end{align*}

Therefore,
\begin{align*}
	\int (1 + \sqrt[3]{x^2})^2 \dif x &= \int (1 + t^2)^2 3t^2 \dif t\\
	&= \int (3t^6 + 6t^4 + 3t^2) \dif t\\
	&= \dfrac{3t^7}{7} + \dfrac{6t^5}{5} + t^3 + c\\
	&= \dfrac{3}{7} (\sqrt[3]{x})^7 + \dfrac{6}{5} (\sqrt[3]{x})^5 + x + c
\end{align*}

\subsection{\[\int \dfrac{x^3 - x}{x^4 - 2x^2 - 7} \dif x\]}

Let
\begin{align*}
	t &= x^4 - 2x^2 - 7\\
	\therefore \dif t &= (4x^3 - 4x) \dif x
\end{align*}

Therefore,
\begin{align*}
	\int \dfrac{x^3 - x}{x^4 - 2x^2 - 7} \dif x &= \dfrac{1}{4} \int \dfrac{\dif t}{t}\\
	&= \dfrac{1}{4} \ln |x^4 - 2x^2 - 7| + c
\end{align*}

\subsection{\[\int \dfrac{1}{\sqrt{9 - x^2}} \dif x\]}

\begin{align*}
	\int \dfrac{1}{\sqrt{9 - x^2}} \dif x &= \dfrac{1}{3} \int \dfrac{1}{\sqrt{1 - (\sfrac{x}{3})^2}} \dif x\\
	&= \sin^{-1} \left( \dfrac{x}{3} \right) + c
\end{align*}

\subsection{\[\int \sin^2 x \dif x\]}

\begin{align*}
	\int \sin^2 x \dif x &= \int \dfrac{1 - \cos(2x)}{2} \dif x\\
	&= \int \dfrac{\dif x}{2} - \int \dfrac{\cos(2x)}{2} \dif x\\
	&= \dfrac{x}{2} - \dfrac{1}{2} \cdot \dfrac{\sin(2x)}{2} + c\\
	&= \dfrac{x}{2} - \dfrac{\sin(2x)}{4} + c
\end{align*}

\subsection{\[\int \tan x \dif x\]}

\begin{align*}
	\int \tan x \dif x &= \int \dfrac{\sin x}{\cos x} \dif x
\end{align*}

Let
\begin{align*}
	t &= \cos x\\
	\therefore \dif t &= -\sin t
\end{align*}

Therefore,
\begin{align*}
	\int \dfrac{\sin x}{\cos x} \dif x &= \int \dfrac{- \dif t}{t}\\
	&= - \ln |t| + c\\
	&= - \ln |\cos x| + c
\end{align*}

\subsection{\[\int x (\ln x)^2 \dif x\]}

Let
\begin{align*}
	x &= e^t\\
	\therefore \dif x &= e^t \dif t
\end{align*}

Therefore,
\begin{align*}
	\int x (\ln x)^2 \dif x &= \int e^t t^2 e^t \dif t\\
	&= \int e^{2t} t^2 \dif t\\
	&= \left( \dfrac{t^2}{2} - \dfrac{t}{2} + \dfrac{1}{4} \right) e^{2t} + c\\
	&= \dfrac{(x \ln x)^2}{2} - \dfrac{x^2 \ln x}{2} + \dfrac{x^2}{4} + c
\end{align*}

\subsection{\[\int x^2 e^x \dif x\]}

\begin{align*}
	\int x^2 e^x \dif x &= x^2 \int e^x \dif x - \int 2x \int e^x \dif x \dif x\\
	&= x^2 e^x - \int 2x e^x \dif x\\
	&= x^2 e^x - 2x \int e^x \dif x + \int 2 \int e^x \dif x \dif x\\
	&= x^2 e^x - 2x e^x + \int 2 e^x \dif x\\
	&= x^2 e^x - 2x e^x + 2 e^x + c
\end{align*}

\subsection{\[\int \dfrac{\ln x}{x^2} \dif x\]}

Let
\begin{align*}
	t &= \ln x\\
	\therefore \dif t &= \dfrac{\dif x}{x}
\end{align*}

Therefore,
\begin{align*}
	\int \dfrac{\ln x}{x^2} \dif x &= \int t e^t \dif t\\
	&= -e^{-t} (t + 1) + c\\
	&= -\dfrac{1}{x} (\ln x + 1) + c 
\end{align*}

\subsection{\[\int x \sinh x \dif x\]}

\begin{align*}
	\int x \sinh x \dif x &= \int x \dfrac{e^x - e^{-x}}{2} \dif x\\
	&= \dfrac{1}{2} \int x (e^x - e^{-x}) \dif x\\
	&= \dfrac{1}{2} \left( (x - 1) e^x + (x + 1) e^{-x} \right) + c
\end{align*}

\section{Solve by substitution}

\subsection{\[\int \dfrac{x}{\sqrt{x^2 + 4}} \dif x\]}

Let
\begin{align*}
	t &= x^2 + 4\\
	\therefore \dif t &= 2x
\end{align*}

Therefore,
\begin{align*}
	\int \dfrac{x}{\sqrt{x^2 + 4}} \dif x &= \int \dfrac{\dif t}{2 \sqrt{t}}\\
	&= \sqrt{t} + c\\
	&= \sqrt{x^2 + 4} + c
\end{align*}

\subsection{\[\int \dfrac{\ln (2x)}{x \ln (4x)} \dif x\]}

Let
\begin{align*}
	t &= \ln (4x)\\
	\therefore t - \ln 2 &= \ln (2x)\\
	\therefore \dif t &= \dfrac{1}{x} \dif x
\end{align*}

Therefore,
\begin{align*}
	\int \dfrac{\ln (2x)}{x \ln (4x)} \dif x &= \int \dfrac{t - \ln 2}{t} \dif t\\
	&= \int \dif t - \int \dfrac{\ln 2}{t} \dif t\\
	&= t - (\ln 2)(\ln t) + c\\
	&= \ln (4x) - (\ln 2)(\ln (\ln 4x)) + c
\end{align*}

\subsection{\[\int \dfrac{x^4}{\sqrt{x^{10} - 2}} \dif x\]}

Let
\begin{align*}
	y &= x^5\\
	\therefore \dif y &= 5 x^4 \dif x
\end{align*}

\begin{align*}
	\therefore \int \dfrac{x^4}{\sqrt{x^{10} - 2}} \dif x &= \dfrac{1}{5} \int \dfrac{\dif y}{\sqrt{y^2 - 2}}\\
	&= \dfrac{1}{5 \sqrt{2}} \int \dfrac{\dif y}{\sqrt{\left( \sfrac{y}{\sqrt{2}} \right)^2 - 1}}
\end{align*}

Let
\begin{align*}
	y &= \dfrac{\sqrt{2}}{\cos z}\\
	\therefore \dif y &= \dfrac{\sqrt{2} \sin z}{\cos^2 z}
\end{align*}

\begin{align*}
	\therefore \int \dfrac{x^4}{\sqrt{x^{10} - 2}} \dif x &= \dfrac{1}{5 \sqrt{2}} \int \dfrac{1}{\sqrt{\sfrac{1}{\cos^2 z} - 1}} \cdot \sqrt{2} \cdot \dfrac{\sin z}{\cos^2 z} \dif z\\
	&= \dfrac{1}{5} \int \dfrac{1}{\tan z} \cdot \dfrac{\sin z}{\cos^2 z} \dif x\\
	&= \dfrac{1}{5} \int \dfrac{1}{\cos z} \dif x\\
	&= \ln |\sec z + \tan z| + c\\
	&= \ln \left\lvert \dfrac{x^5 + \sqrt{x^{10} - 2}}{\sqrt{2}} \right\rvert + c
\end{align*}

\subsection{\[\int \dfrac{1}{x \sqrt{2x + 1}} \dif x\]}

Let
\begin{align*}
	t &= \sqrt{2x + 1}\\
	\therefore \dif t &= x \dif x
\end{align*}

\begin{align*}
	\int \dfrac{1}{x \sqrt{2x + 1}} \dif x &= \int \dfrac{t \dif t}{\frac{t^2 - 1}{2} \cdot t}\\
	&= \int \dfrac{2 \dif t}{(t + 1)(t - 1)}\\
	&= \int \left( \dfrac{1}{t - 1} - \dfrac{1}{t + 1} \right) \dif t\\
	&= \ln \left\lvert \dfrac{t - 1}{t + 1} \right\rvert + c\\
	&= \ln \left\lvert \dfrac{\sqrt{2x + 1} - 1}{\sqrt{2x + 1} + 1} \right\rvert + c
\end{align*}

\section{Solve the following integrals}

\subsection{\[\int \cos(7x) \sin(7x) \dif x\]}

\begin{align*}
	\int \cos(7x) \sin(7x) \dif x &= \dfrac{1}{2} \int \sin(14x) \dif x\\
	&= \dfrac{1}{2} \left( -\dfrac{\cos (14x)}{14} \right) + c\\
	&= \dfrac{\cos (14x)}{28} + c
\end{align*}

\subsection{\[\int \cos(3x) \cos(2x) \dif x\]}

\begin{align*}
	\int \cos(3x) \cos(2x) \dif x &= \int (\cos(5x) + \cos(x)) \dif x\\
	&= -\dfrac{\sin(5x)}{5} + \sin x + c
\end{align*}

\subsection{\[\int \dfrac{1}{\cos x + \sin x + 1} \dif x\]}

\begin{align*}
	\int \dfrac{1}{\cos x + \sin x + 1} \dif x &= \int \dfrac{1}{2 \cos^2 (\sfrac{x}{2}) + 2 \sin (\sfrac{x}{2}) \cos (\sfrac{x}{2})} \dif x\\
	&= \int \dfrac{1}{2 \cos^2 (\sfrac{x}{2}) (1 + \tan (\sfrac{x}{2}))} \dif x\\
	&= \int \dfrac{\sec^2 (\sfrac{x}{2})}{1 + \tan (\sfrac{x}{2})} \dif x\\
	&= \ln \left\lvert 1 + \tan (\sfrac{x}{2}) \right\rvert + c
\end{align*}

\subsection{\[\int \dfrac{1}{\sin x} \dif x\]}

\begin{align*}
	\int \csc x \dif x &= \int \dfrac{\csc x (\csc x + \cot x)}{\csc x + \cot x} \dif x
\end{align*}

Let
\begin{align*}
	t &= \csc x + \cot x\\
	\therefore \dif t &= -\csc x \cot x -\csc^2 x \dif x
\end{align*}

Therefore,
\begin{align*}
	\int \dfrac{\csc x (\csc x + \cot x)}{\csc x + \cot x} \dif x &= \int -\dfrac{\dif t}{t}\\
	&= -\ln |t| + c\\
	&= -\ln |\csc x + \cot x| + c
\end{align*}

\subsection{\[\int \dfrac{1}{1 - \sin x} \dif x\]}

\begin{align*}
	\int \dfrac{1}{1 - \sin x} \dif x &= \int \dfrac{1 + \sin x}{1 - \sin^2 x} \dif x\\
	&= \int \dfrac{1 + \sin x}{\cos x} \dif x\\
	&= \int \dfrac{1}{\cos^2 x} \dif x + \int \dfrac{\sin x}{\cos^2 x} \dif x\\
	&= \tan x + \sec x + c
\end{align*}

\subsection{\[\int \sin^2 x \cos^4 x \dif x\]}

\begin{align*}
	\int \sin^2 x \cos^4 x \dif x &= \int \dfrac{1 - \cos (2x)}{2} \left( \dfrac{1 + \cos (2x)}{2} \right)^2 \dif x\\
	&= \dfrac{1}{8} \int (1 - \cos^2 (2x))(1 + \cos (2x)) \dif x\\
	&= \dfrac{1}{8} \int \left( \dfrac{1 - \cos (4x)}{2} \right) \dif x + \int \sin^2 (2x) \cos (2x) \dif x\\
	&= \dfrac{1}{16} \left( x - \dfrac{\sin (4x)}{4} + \dfrac{\sin^3 (2x)}{3} \right) + c
\end{align*}

\subsection{\[\int \dfrac{\sin (2x)}{\sqrt{3 - \cos^4 x}} \dif x\]}

\begin{align*}
	\int \dfrac{\sin (2x)}{\sqrt{3 - \cos^4 x}} \dif x &= \int \dfrac{2 \sin x \cos x}{\sqrt{3 - \cos^4 x}} \dif x
\end{align*}

Let
\begin{align*}
	t^2 &= 3 - \cos^4 x\\
	\therefore 2 \sin x \cos x \dif x &= \dfrac{t \dif t}{\sqrt{3 - t^2}}
\end{align*}

Therefore,
\begin{align*}
	\int \dfrac{2 \sin x \cos x}{\sqrt{3 - \cos^4 x}} \dif x &= \int \dfrac{t \dif t}{t \sqrt{3 - t^2}}\\
	&= \sin^{-1} \dfrac{t}{\sqrt{3}} + c\\
	&= \sin^{-1} \sqrt{\dfrac{3 - \cos^4 x}{3}} + c
\end{align*}

\subsection{\[\int e^{4x} \cos (2x) \dif x\]}

\begin{align*}
	\int e^{4x} \cos (2x) \dif x &= e^{4x} \int \cos (2x) \dif x - \int 4e^{4x} \int \cos (2x) \dif x \dif x\\
	&= \dfrac{e^{4x} \sin (2x)}{2} - \int 2e^{4x} \sin (2x) \dif x\\
	&= \dfrac{e^{4x} \sin (2x)}{2} - \left( 2e^{4x} \int \sin(2x) \dif x - \int 8e^{4x} \int \sin (2x) \dif x \dif x \right)\\
	&= \dfrac{e^{4x} \sin (2x)}{2} - \left( - e^{4x} \cos(2x) + 4 \int e^{4x} \cos (2x) \dif x \right)\\
	&= \dfrac{e^{4x} \sin (2x)}{2} + e^{4x} \cos(2x) - 4 \int e^{4x} \cos (2x) \dif x\\
	\therefore 5 \int e^{4x} \cos (2x) \dif x &= \dfrac{e^{4x} \sin (2x)}{2} + e^{4x} \cos (2x)\\
	\therefore \int e^{4x} \cos (2x) \dif x &= \dfrac{1}{5} \left( \dfrac{e^{4x} \sin (2x)}{2} + e^{4x} \cos (2x) \right)\\
\end{align*}

\subsection{\[\int \ln x \dif x\]}

\begin{align*}
	\int \ln x \dif x &= \int 1 \cdot \ln x \dif x\\
	&= \ln x \int 1 \cdot \dif x - \int \dfrac{1}{x} \int 1 \cdot \dif x \dif x\\
	&= x \ln x - x + c
\end{align*}

\subsection{\[\int \dfrac{1}{x (\ln x)^x}\]}

Let
\begin{align*}
	t &= \ln x\\
	\therefore \dif t &= \dfrac{1}{x} \dif x
\end{align*}

Therefore,
\begin{align*}
	\int \dfrac{1}{x (\ln x)^x} &= \int \dfrac{\dif t}{t^2}\\
	&= -\dfrac{1}{t} + c\\
	&= -\dfrac{1}{\ln x} + c
\end{align*}

\subsection{\[\int \dfrac{1}{\sqrt{x}(1 + \sqrt[3]{x})} \dif x\]}

Let
\begin{align*}
	x &= t^6\\
	\therefore \dif x &= 6t^5 \dif t
\end{align*}

Therefore,
\begin{align*}
	\int \dfrac{1}{\sqrt{x}(1 + \sqrt[3]{x})} \dif x &= \int \dfrac{6t^5}{t^3(1 + t^2)} \dif t\\
	&= \int \dfrac{6t^2}{(1 + t^2)} \dif t\\
	&= \int \dfrac{6(t^2 + 1) - 6}{(t^2 + 1)} \dif t\\
	&= \int 6 \dif t - \int \dfrac{6}{t^2 + 1} \dif t\\
	&= 6t - 6 \tan^{-1} t + c\\
	&= 6\sqrt[6]{x} + 6 \tan^{-1} \sqrt[6]{x} + c
\end{align*}

\subsection{\[\int \dfrac{1}{x^2 - 1} \dif x\]}

\begin{align*}
	\int \dfrac{1}{x^2 - 1} &= \dfrac{1}{2} \int \left( \dfrac{1}{x - 1} - \dfrac{1}{x + 1} \right) \dif x\\
	&= \dfrac{1}{2} \ln \left\lvert \dfrac{x - 1}{x + 1} \right\rvert + c
\end{align*}

\subsection{\[\int \dfrac{x^3 - 1}{4x^3 - x} \dif x\]}

\begin{align*}
	\int \dfrac{x^3 - 1}{4x^3 - x} \dif x &= \dfrac{1}{4} \int \dfrac{4x^3 - x + x - 4}{4x^3 - x} \dif x\\
	&= \dfrac{1}{4} \int \dfrac{4x^3 - x}{4x^3 - x} \dif x - \int \dfrac{4 - x}{4x^3 - x} \dif x\\
	&= \dfrac{1}{4} \left( x + \int \dfrac{4}{x} - \dfrac{7}{2(2x - 1)} - \dfrac{9}{2(2x + 1)} \dif x \right)\\
	&= \dfrac{1}{4} \left( x + 4 \ln |x| + \dfrac{7}{4} \ln |2x - 1| - \dfrac{9}{4} \ln |2x + 1| \right)
\end{align*}

\subsection{\[\int \dfrac{1}{x(x + 1)^2} \dif x\]}

\begin{align*}
	\int \dfrac{1}{x(x + 1)^2} \dif x &= \int \left( \dfrac{1}{x} - \dfrac{1}{x +1} -\dfrac{1}{(x + 1)^2} \right) \dif x\\
	&= \ln \left\lvert \dfrac{x}{x + 1} \right\rvert + \dfrac{1}{x + 1} + c
\end{align*}

\subsection{\[\int \dfrac{x^2}{(x - 1)^5} \dif x\]}

Let
\begin{align*}
	t &= x - 1\\
	\therefore x &= t + 1\\
	\therefore \dif t &= \dif x
\end{align*}

\begin{align*}
	\int \dfrac{x^2}{(x - 1)^5} \dif x &= \int \dfrac{(t + 1)^2}{t^5} \dif x\\
	&= \int \dfrac{t^2 + 2t + 1}{t^5} \dif t\\
	&= \int \left( \dfrac{1}{t^3} + \dfrac{2}{t^4} + \dfrac{1}{t^5} \right) \dif t\\
	&= -\dfrac{1}{2x^2} - \dfrac{2}{3x^3} - \dfrac{1}{4x^4} + c
\end{align*}

\end{document}