\documentclass[fleqn, 12pt]{article}
\setcounter{secnumdepth}{4}
\usepackage{amsmath, amssymb, amsthm}
\usepackage{commath, esdiff}
\usepackage{datetime}
\usepackage{graphicx, epstopdf}
\usepackage{ulem}
\usepackage{xfrac}
\usepackage{enumerate}
\usepackage{tikz}

\newcommand\numberthis{\addtocounter{equation}{1}\tag{\theequation}}

\theoremstyle{definition}
\newtheorem{example}{Example}
\newtheorem{definition}{Definition}

\theoremstyle{theorem}
\newtheorem{theorem}{Theorem}

\newenvironment{solution}
{\begin{proof}[Solution]\let\qed\relax}
	{\end{proof}}

%opening
\title{Recitation 14}
\author{Aakash Jog}
\date{\formatdate{21}{1}{2015}}

\begin{document}

\maketitle
%\setlength{\mathindent}{0pt}

\tableofcontents

\newpage
\section{Double Integrals}

\begin{example}
	Calculate $\displaystyle \iint\limits_{D} y \dif x \dif y$ where $D$ is bounded by $x = y^2, y \geq 0$ and $y = x^2$.
\end{example}

\begin{solution}
	\begin{align*}
		\iint\limits_D y \dif x \dif y &= \int\limits_{0}^{1} \int\limits_{x^2}^{\sqrt{x}} y \dif y \dif x\\
		&= \int\limits_{0}^{1} \left. \dfrac{y^2}{2} \right|_{y = x^2}^{y = \sqrt{x}} \dif x\\
		&= \int\limits_{0}^{1} \left( \dfrac{x}{2} - \dfrac{x^4}{2} \right) \dif x\\
		&= \left. \dfrac{x^2}{4} - \dfrac{x^5}{10} \right|_{0}^{1}\\
		&= \dfrac{1}{4} - \dfrac{1}{10}\\
		&= \dfrac{3}{20}
	\end{align*}
\end{solution}

\section{Triple Integrals}

\begin{example}
	Find $\displaystyle \iiint\limits_{E} x^2 + y^2 + z^2 \dif V$ where $E$ is bounded by $x = 0$, $y = 0$, $z = 0$ and $x + y + z = a, a > 0$.
\end{example}

\begin{solution}
	\begin{tikzpicture}
		\def\a{2};

		\begin{scope}[-stealth]
			\draw (0,0,0) -- ({\a+1},0,0);
			\draw (0,0,0) -- (0,{\a+1},0);
			\draw (0,0,0) -- (0,0,{\a+1});
		\end{scope}

		\begin{scope}
			\draw (\a,0,0) -- (0,\a,0) -- (0,0,\a) -- cycle;
		\end{scope}
	\end{tikzpicture}
	Therefore,
	\begin{align*}
		\iiint\limits_{E} x^2 + y^2 + z^2 \dif V &= \int\limits_{0}^{a} \int\limits_{0}^{a - x} \int\limits_{0}^{a - x - y} x^2 + y^2 + z^2 \dif z \dif y \dif x
	\end{align*}
\end{solution}

\begin{example}
	Calculate $\displaystyle \iiint\limits_{E} x e^z \dif V$ where $E$ is bounded by $z = x^2 + y^2$ and $z = 8 - x^2 - y^2$.
\end{example}

\begin{solution}
	The two boundaries intersect at $x^2 + y^2 = 4$. Therefore the projection of the volume is the circle.\\
	Therefore,
	\begin{align*}
		\iiint\limits_{E} x e^z \dif V &= \int\limits_{-2}^{2} \int\limits_{-\sqrt{4 - x^2}}^{\sqrt{4 - x^2}} \int\limits_{x^2 + y^2}^{8 - x^2 - y^2} x e^z \dif z \dif y \dif x
	\end{align*}
\end{solution}

\section{Line Integrals of Scalar Functions}

\begin{example}
	Calculate $\displaystyle \int\limits_{C} x^2 + y^2 \dif s$ where $C$ is a circle of radius 2.
\end{example}

\begin{solution}
	\begin{align*}
		\int\limits_{C} x^2 + y^2 \dif s &= \int\limits_{0}^{2 \pi} \left( (2 \cos t)^2 + (2 \sin t)^2 \right) \cdot 2 \dif t\\
		&= 16 \pi
	\end{align*}
\end{solution}

\section{Line Integrals of Vector Functions}

\begin{example}
	Calculate $\displaystyle \int\limits_{C} \dfrac{x}{y} \dif x + \dfrac{y - x}{x} \dif y$ where $C$ is the path over the parabola $y = x^2$ from $(2,4)$ to $(1,1)$.
\end{example}

\begin{solution}
	\begin{align*}
		\int\limits_{C} \left( \dfrac{x}{y}, \dfrac{y - x}{x} \right) \dif r &= \int\limits_{2}^{1} \left( \dfrac{t}{t^2} + \dfrac{t^2 - t}{t} \right) \cdot (1, 2t) \dif t\\
		&= \int\limits_{2}^{1} \left( \dfrac{1}{t} + (t - 1) \cdot 2t \right) \dif t\\
		&= \left. \ln t + \dfrac{2 t^3}{3} - t^2 \right|_{2}^{1}\\
		&= \ln \dfrac{1}{2} + \dfrac{2}{3} - \dfrac{16}{3} - 1 + 4\\
		&= 3 - \dfrac{14}{3} - \ln 2\\
		&= \dfrac{5}{3} - \ln 2
	\end{align*}
\end{solution}

\end{document}